experiment/Experiment.Steel.Repr.SF.fsti
@@ -1,4 +1,4 @@
-module Experiment.Steel.Repr.Fun
+module Experiment.Steel.Repr.SF
 
 module U   = Learn.Util
 module L   = FStar.List.Pure
@@ -111,7 +111,7 @@ let mk_prog_shape (#a : Type) (#post : post_t a) (t : prog_tree a post)
   { post_len; shp}
 
 
-(*** Repr.ST --> Repr.Fun *)
+(*** Repr.ST --> Repr.SF *)
 
 module Opt = Learn.Option
 
@@ -172,210 +172,210 @@ let post_src_of_shape
 
 noeq
 type post_bij_t' (#pre_n : nat) (#post_n : nat) (s : post_src_f pre_n post_n) = {
-  len_Fun : nat;
-  idx_Fun : (i : Fin.fin post_n {None? (s i)}) -> Fin.fin len_Fun;
-  idx_ST  : Fin.fin len_Fun -> (i : Fin.fin post_n  {None? (s i)});
+  len_SF : nat;
+  idx_SF : (i : Fin.fin post_n {None? (s i)}) -> Fin.fin len_SF;
+  idx_ST  : Fin.fin len_SF -> (i : Fin.fin post_n  {None? (s i)});
 }
 
 type post_bij_t (#pre_n : nat) (#post_n : nat) (s : post_src_f pre_n post_n) =
   r : post_bij_t' s {
-    (forall (i : Fin.fin post_n {None? (s i)}) . {:pattern (r.idx_ST (r.idx_Fun i))}
-      r.idx_ST (r.idx_Fun i) = i) /\
-    (forall (j : Fin.fin r.len_Fun) . {:pattern (r.idx_Fun (r.idx_ST j))}
-      r.idx_Fun (r.idx_ST j) = j)
+    (forall (i : Fin.fin post_n {None? (s i)}) . {:pattern (r.idx_ST (r.idx_SF i))}
+      r.idx_ST (r.idx_SF i) = i) /\
+    (forall (j : Fin.fin r.len_SF) . {:pattern (r.idx_SF (r.idx_ST j))}
+      r.idx_SF (r.idx_ST j) = j)
   }
 
 let rec mk_post_bij (#pre_n : nat) (#post_n : nat) (s : post_src_f pre_n post_n)
   : Tot (post_bij_t s) (decreases post_n)
   = if post_n = 0 then {
-       len_Fun = 0;
-       idx_Fun = (fun _ -> false_elim ());
+       len_SF = 0;
+       idx_SF = (fun _ -> false_elim ());
        idx_ST  = (fun _ -> false_elim ())}
     else
       let s' : post_src_f pre_n (post_n - 1) = fun i -> s (i+1) in
       let p' = mk_post_bij s' in
       match s 0 with
-      | Some _ -> { len_Fun = p'.len_Fun;
-                   idx_Fun = (fun i -> p'.idx_Fun (i-1));
-                   idx_ST  = (fun j -> p'.idx_ST j + 1)}
-      | None   -> { len_Fun = p'.len_Fun + 1;
-                   idx_Fun = (fun i -> if i = 0 then 0 else (p'.idx_Fun (i-1) + 1));
-                   idx_ST  = (fun j -> if j = 0 then 0 else (p'.idx_ST (j-1) + 1))}
+      | Some _ -> { len_SF = p'.len_SF;
+                   idx_SF = (fun i -> p'.idx_SF (i-1));
+                   idx_ST = (fun j -> p'.idx_ST j + 1)}
+      | None   -> { len_SF = p'.len_SF + 1;
+                   idx_SF = (fun i -> if i = 0 then 0 else (p'.idx_SF (i-1) + 1));
+                   idx_ST = (fun j -> if j = 0 then 0 else (p'.idx_ST (j-1) + 1))}
 
 let rec post_bij (#post_n : nat) (#pre_n : nat) (s : ST.shape_tree pre_n post_n)
   : Tot (post_bij_t (post_src_f_of_shape s)) (decreases s)
   = match s with
   | ST.Sequiv n p ->
-           { len_Fun = 0; idx_Fun = (fun _ -> false_elim ()); idx_ST = (fun _ -> false_elim ()) }
+           { len_SF = 0; idx_SF = (fun _ -> false_elim ()); idx_ST = (fun _ -> false_elim ()) }
   | ST.Sframe pre_n post_n frame_n f ->
            let bj = post_bij f in
-           { len_Fun = bj.len_Fun;
-             idx_Fun = (fun (i : Fin.fin (post_n + frame_n) {None? (post_src_f_of_shape s i)}) -> bj.idx_Fun i);
-             idx_ST  = bj.idx_ST }
+           { len_SF = bj.len_SF;
+             idx_SF = (fun (i : Fin.fin (post_n + frame_n) {None? (post_src_f_of_shape s i)}) -> bj.idx_SF i);
+             idx_ST = bj.idx_ST }
   | ST.Sspec  pre_n post_n ->
-           { len_Fun = post_n; idx_Fun = (fun i -> i); idx_ST = (fun j -> j) }
+           { len_SF = post_n; idx_SF = (fun i -> i); idx_ST = (fun j -> j) }
   | ST.Sret   _ n ->
-           { len_Fun = n; idx_Fun = (fun i -> i); idx_ST = (fun j -> j) }
+           { len_SF = n; idx_SF = (fun i -> i); idx_ST = (fun j -> j) }
   | ST.Sbind  pre_n itm_n post_n f g ->
-           { len_Fun = post_n; idx_Fun = (fun i -> i); idx_ST = (fun j -> j) }
+           { len_SF = post_n; idx_SF = (fun i -> i); idx_ST = (fun j -> j) }
   | ST.SbindP pre_n post_n g ->
-           { len_Fun = post_n; idx_Fun = (fun i -> i); idx_ST = (fun j -> j) }
+           { len_SF = post_n; idx_SF = (fun i -> i); idx_ST = (fun j -> j) }
 
 
-let postl_Fun_of_ST
+let postl_SF_of_ST
       (post : Fl.ty_list)
       (#pre_n : nat) (#s : post_src_f pre_n (L.length post)) (bij : post_bij_t s)
   : Fl.ty_list
-  = Ll.initi 0 bij.len_Fun (fun i -> L.index post (bij.idx_ST i))
+  = Ll.initi 0 bij.len_SF (fun i -> L.index post (bij.idx_ST i))
 
-let post_Fun_of_ST
+let post_SF_of_ST
       (#a : Type u#a) (post : ST.post_t u#a u#b a)
       (#pre_n #post_n : nat) (s : ST.shape_tree pre_n post_n {post_has_len post post_n})
   : post_t u#a u#b a
-  = fun (x : a) -> postl_Fun_of_ST (post x) (post_bij s)
+  = fun (x : a) -> postl_SF_of_ST (post x) (post_bij s)
 
-let sell_Fun_of_ST
+let sell_SF_of_ST
       (post : Fl.ty_list)
       (#pre_n : nat) (#s : post_src_f pre_n (L.length post)) (bij : post_bij_t s)
       (sl_ST : Fl.flist post)
-  : Fl.flist (postl_Fun_of_ST post bij)
+  : Fl.flist (postl_SF_of_ST post bij)
   = 
-    Fl.mk_flist (postl_Fun_of_ST post bij)
-                (fun i -> U.cast (L.index (postl_Fun_of_ST post bij) i) (sl_ST (bij.idx_ST i)))
+    Fl.mk_flist (postl_SF_of_ST post bij)
+                (fun i -> U.cast (L.index (postl_SF_of_ST post bij) i) (sl_ST (bij.idx_ST i)))
 
-let sel_Fun_of_ST
+let sel_SF_of_ST
       (#a : Type u#a) (post : ST.post_t u#a u#b a)
       (#pre_n #post_n : nat) (s : ST.shape_tree pre_n post_n {post_has_len post post_n})
       (x : a)
-  : Fl.flist (post x) -> post_v (post_Fun_of_ST post s) x
-  = sell_Fun_of_ST (post x) (post_bij s)
+  : Fl.flist (post x) -> post_v (post_SF_of_ST post s) x
+  = sell_SF_of_ST (post x) (post_bij s)
 
 unfold
-let return_Fun_post_of_ST
+let return_SF_post_of_ST
       (#a : Type u#a) (post : ST.post_t u#a u#b a)
       (#pre_n #post_n : nat) (s : ST.shape_tree pre_n post_n {post_has_len post post_n})
       (x : a) (post_val : Fl.flist (post x))
-  : prog_tree a (post_Fun_of_ST post s)
-  = Tret a x (post_Fun_of_ST post s) (Fl.dlist_of_f (sel_Fun_of_ST post s x post_val))
+  : prog_tree a (post_SF_of_ST post s)
+  = Tret a x (post_SF_of_ST post s) (Fl.dlist_of_f (sel_SF_of_ST post s x post_val))
 
 
-let sell_ST_of_Fun
+let sell_ST_of_SF
       (#pre #post : Fl.ty_list)
       (s : post_src pre post) (bij : post_bij_t s)
-      (sl0 : Fl.flist pre) (sl1_Fun : Fl.flist (postl_Fun_of_ST post bij))
+      (sl0 : Fl.flist pre) (sl1_SF : Fl.flist (postl_SF_of_ST post bij))
   : Fl.flist post
   =
     Fl.mk_flist post
          (fun i -> match s i with
                 | Some j -> U.cast (L.index post i) (sl0 j)
-                | None   -> U.cast (L.index post i) (sl1_Fun (bij.idx_Fun i)))
+                | None   -> U.cast (L.index post i) (sl1_SF (bij.idx_SF i)))
 
-let sel_ST_of_Fun
+let sel_ST_of_SF
       (#a : Type) (#pre : ST.pre_t) (#post : ST.post_t a) (t : ST.prog_tree a pre post)
       (s : ST.prog_shape t)
-      (sl0 : Fl.flist pre) (x : a) (sl1_Fun : post_v (post_Fun_of_ST post s.shp) x)
+      (sl0 : Fl.flist pre) (x : a) (sl1_SF : post_v (post_SF_of_ST post s.shp) x)
   : Fl.flist (post x)
-  = sell_ST_of_Fun (post_src_of_shape t s x) (post_bij s.shp) sl0 sl1_Fun
+  = sell_ST_of_SF (post_src_of_shape t s x) (post_bij s.shp) sl0 sl1_SF
 
-val sell_Fun_ST_Fun
+val sell_SF_ST_SF
       (#pre #post : Fl.ty_list)
       (s : post_src pre post) (bij : post_bij_t s)
-      (sl0 : Fl.flist pre) (sl1_Fun : Fl.flist (postl_Fun_of_ST post bij))
-  : Lemma (sell_Fun_of_ST post bij (sell_ST_of_Fun s bij sl0 sl1_Fun) == sl1_Fun)
+      (sl0 : Fl.flist pre) (sl1_SF : Fl.flist (postl_SF_of_ST post bij))
+  : Lemma (sell_SF_of_ST post bij (sell_ST_of_SF s bij sl0 sl1_SF) == sl1_SF)
 
-let sel_Fun_ST_Fun
+let sel_SF_ST_SF
       (#a : Type) (#pre : ST.pre_t) (#post : ST.post_t a) (t : ST.prog_tree a pre post)
       (s : ST.prog_shape t)
-      (sl0 : Fl.flist pre) (x : a) (sl1_Fun : post_v (post_Fun_of_ST post s.shp) x)
-  : Lemma (sel_Fun_of_ST post s.shp x (sel_ST_of_Fun t s sl0 x sl1_Fun) == sl1_Fun)
-  = sell_Fun_ST_Fun (post_src_of_shape t s x) (post_bij s.shp) sl0 sl1_Fun
+      (sl0 : Fl.flist pre) (x : a) (sl1_SF : post_v (post_SF_of_ST post s.shp) x)
+  : Lemma (sel_SF_of_ST post s.shp x (sel_ST_of_SF t s sl0 x sl1_SF) == sl1_SF)
+  = sell_SF_ST_SF (post_src_of_shape t s x) (post_bij s.shp) sl0 sl1_SF
 
 
-val post_Fun_of_ST__frame
+val post_SF_of_ST__frame
       (#a : Type) (post : ST.post_t a) (frame: Fl.ty_list)
       (pre_n : nat) (post_n : nat {post_has_len post post_n}) (f : ST.shape_tree pre_n post_n)
-  : Lemma (post_Fun_of_ST (ST.frame_post post frame) (Sframe pre_n post_n (L.length frame) f)
-                == post_Fun_of_ST post f)
+  : Lemma (post_SF_of_ST (ST.frame_post post frame) (Sframe pre_n post_n (L.length frame) f)
+                == post_SF_of_ST post f)
 
-val post_Fun_of_ST__spec
+val post_SF_of_ST__spec
       (#a : Type) (post : ST.post_t a)
       (pre_n : nat) (post_n : nat {post_has_len post post_n})
-  : Lemma (post_Fun_of_ST post (ST.Sspec pre_n post_n) == U.eta post)
+  : Lemma (post_SF_of_ST post (ST.Sspec pre_n post_n) == U.eta post)
 
-val post_Fun_of_ST__ret
+val post_SF_of_ST__ret
       (#a : Type) (post : ST.post_t a) (smp_ret : bool) (post_n : nat {post_has_len post post_n})
-  : Lemma (post_Fun_of_ST post (ST.Sret smp_ret post_n) == U.eta post)
+  : Lemma (post_SF_of_ST post (ST.Sret smp_ret post_n) == U.eta post)
 
 
-let rec repr_Fun_of_ST
+let rec repr_SF_of_ST
       (#a : Type u#a) (#pre : ST.pre_t u#b) (#post : ST.post_t u#a u#b a)
       (t : ST.prog_tree a pre post)
-  : Tot ((s : ST.prog_shape t) -> Fl.flist pre -> prog_tree a (post_Fun_of_ST post s.shp))
+  : Tot ((s : ST.prog_shape t) -> Fl.flist pre -> prog_tree a (post_SF_of_ST post s.shp))
         (decreases t)
   = match t as t'
       returns (s : ST.prog_shape t) -> Fl.flist pre ->
-              prog_tree a (post_Fun_of_ST post s.shp)
+              prog_tree a (post_SF_of_ST post s.shp)
     with
     | ST.Tequiv pre post0 p -> fun s sl0 ->
             Tret U.unit' U.Unit' (fun _ -> []) Dl.DNil
     | ST.Tframe a pre post frame f -> fun s sl0 ->
             (**) let ST.Sframe _ post_n _ shp_f = s.shp in
-            (**) post_Fun_of_ST__frame post frame (L.length pre) post_n shp_f;
+            (**) post_SF_of_ST__frame post frame (L.length pre) post_n shp_f;
             let sl0' : Fl.flist pre = (Fl.splitAt_ty pre frame sl0)._1 in
-            repr_Fun_of_ST f (ST.mk_prog_shape f shp_f) sl0'
+            repr_SF_of_ST f (ST.mk_prog_shape f shp_f) sl0'
     | ST.Tspec a pre post req ens -> fun s sl0 ->
             (**) let ST.Sspec _ post_n = s.shp in
-            (**) post_Fun_of_ST__spec post (L.length pre) post_n;
+            (**) post_SF_of_ST__spec post (L.length pre) post_n;
             Tspec a (U.eta post) (req sl0) (ens sl0)
     | ST.Tret a x post -> fun s sl ->
             (**) let ST.Sret smp_ret post_n = s.shp in
-            (**) post_Fun_of_ST__ret post smp_ret post_n;
+            (**) post_SF_of_ST__ret post smp_ret post_n;
             Tret a x (U.eta post) (Fl.dlist_of_f sl)
     | ST.Tbind a b pre itm post f g -> fun s sl0 ->
             (**) let ST.Sbind _ itm_n post_n shp_f shp_g = s.shp in
             (**) let s_f = ST.mk_prog_shape f shp_f in
-            Tbind a b  _ _ (repr_Fun_of_ST f s_f sl0) (fun x sl1' ->
+            Tbind a b  _ _ (repr_SF_of_ST f s_f sl0) (fun x sl1' ->
             (**) let s_g : ST.prog_shape (g x) = ST.mk_prog_shape (g x) shp_g in
-            let sl1 = sel_ST_of_Fun f s_f sl0 x sl1' in
-            Tbind b b  (post_Fun_of_ST post #(L.length (itm x)) shp_g) _
-                       (repr_Fun_of_ST (g x) s_g sl1) (fun y sl2' ->
-            let sl2 = sel_ST_of_Fun (g x) s_g sl1 y sl2' in
-            return_Fun_post_of_ST post s.shp y sl2))
+            let sl1 = sel_ST_of_SF f s_f sl0 x sl1' in
+            Tbind b b  (post_SF_of_ST post #(L.length (itm x)) shp_g) _
+                       (repr_SF_of_ST (g x) s_g sl1) (fun y sl2' ->
+            let sl2 = sel_ST_of_SF (g x) s_g sl1 y sl2' in
+            return_SF_post_of_ST post s.shp y sl2))
     | ST.TbindP a b pre post wp f g -> fun s sl0 ->
             (**) let ST.SbindP _ post_n shp_g = s.shp in
             TbindP a b _ wp f (fun x ->
             (**) let s_g : ST.prog_shape (g x) = ST.mk_prog_shape (g x) shp_g in
-            Tbind  b b (post_Fun_of_ST post #(L.length #Type pre) shp_g) _
-                       (repr_Fun_of_ST (g x) s_g sl0) (fun y sl1' ->
-            let sl1 = sel_ST_of_Fun (g x) s_g sl0 y sl1' in
-            return_Fun_post_of_ST post s.shp y sl1))
+            Tbind  b b (post_SF_of_ST post #(L.length #Type pre) shp_g) _
+                       (repr_SF_of_ST (g x) s_g sl0) (fun y sl1' ->
+            let sl1 = sel_ST_of_SF (g x) s_g sl0 y sl1' in
+            return_SF_post_of_ST post s.shp y sl1))
 
 
-let rec shape_Fun_of_ST
+let rec shape_SF_of_ST
       (#pre_n #post_n : nat) (t : ST.shape_tree pre_n post_n)
-  : Tot (shape_tree (post_bij t).len_Fun) (decreases t)
+  : Tot (shape_tree (post_bij t).len_SF) (decreases t)
   = match t with
     | ST.Sequiv _ _ ->
             Sret true 0
     | ST.Sframe pre_n post_n frame_n s_f ->
-            shape_Fun_of_ST s_f
+            shape_SF_of_ST s_f
     | ST.Sspec pre_n post_n ->
             Sspec post_n
     | ST.Sret smp_ret n ->
             Sret smp_ret n
     | ST.Sbind pre_n itm_n post_n s_f s_g ->
-            Sbind _ _ (shape_Fun_of_ST s_f) (
-            Sbind _ _ (shape_Fun_of_ST s_g)
+            Sbind _ _ (shape_SF_of_ST s_f) (
+            Sbind _ _ (shape_SF_of_ST s_g)
                       (Sret true post_n))
     | ST.SbindP pre_n post_n s_g ->
-            SbindP _ (Sbind _ _ (shape_Fun_of_ST s_g) (Sret true post_n))
+            SbindP _ (Sbind _ _ (shape_SF_of_ST s_g) (Sret true post_n))
 
 
 (**) val __end_repr_fun_of_st : unit
 #pop-options
 
 
-(***** soundness of ST --> Fun *)
+(***** soundness of ST --> SF *)
 
 // TODO? pattern
 let post_eq_src (#pre #post : Fl.ty_list) (s : post_src pre post)
@@ -394,34 +394,34 @@ let post_eq_srcD
                 sl1_ST i == U.cast (L.index post i) (sl0 (Some?.v (s i)))
       with i
 
-val sell_ST_of_Fun_eq_src
+val sell_ST_of_SF_eq_src
       (#pre #post : Fl.ty_list)
       (s : post_src pre post) (bij : post_bij_t s)
-      (sl0 : Fl.flist pre) (sl1_Fun : Fl.flist (postl_Fun_of_ST post bij))
-  : Lemma (post_eq_src s sl0 (sell_ST_of_Fun s bij sl0 sl1_Fun))
+      (sl0 : Fl.flist pre) (sl1_SF : Fl.flist (postl_SF_of_ST post bij))
+  : Lemma (post_eq_src s sl0 (sell_ST_of_SF s bij sl0 sl1_SF))
 
-val post_eq_src_ST_Fun_ST
+val post_eq_src_ST_SF_ST
       (#pre #post : Fl.ty_list)
       (s : post_src pre post) (bij : post_bij_t s)
       (sl0 : Fl.flist pre) (sl1_ST : Fl.flist post)
   : Lemma (requires post_eq_src s sl0 sl1_ST)
-          (ensures  sell_ST_of_Fun s bij sl0 (sell_Fun_of_ST post bij sl1_ST) == sl1_ST)
+          (ensures  sell_ST_of_SF s bij sl0 (sell_SF_of_ST post bij sl1_ST) == sl1_ST)
 
 (* TODO? def de post_eq_src *)
 let post_eq_src_iff
       (#pre #post : Fl.ty_list) (s : post_src pre post) (bij : post_bij_t s)
       (sl0 : Fl.flist pre) (sl1_ST : Fl.flist post)
   : Lemma (post_eq_src s sl0 sl1_ST
-           <==> sl1_ST == sell_ST_of_Fun s bij sl0 (sell_Fun_of_ST post bij sl1_ST))
-  = sell_ST_of_Fun_eq_src s bij sl0 (sell_Fun_of_ST post bij sl1_ST);
-    FStar.Classical.move_requires (post_eq_src_ST_Fun_ST s bij sl0) sl1_ST
+           <==> sl1_ST == sell_ST_of_SF s bij sl0 (sell_SF_of_ST post bij sl1_ST))
+  = sell_ST_of_SF_eq_src s bij sl0 (sell_SF_of_ST post bij sl1_ST);
+    FStar.Classical.move_requires (post_eq_src_ST_SF_ST s bij sl0) sl1_ST
 
 
 unfold
 let req_equiv #a #pre #post (t : ST.prog_tree a pre post) (s : ST.prog_shape t)
       (sl0 : Fl.flist pre)
   : prop
-  = ST.tree_req t sl0 <==> tree_req (repr_Fun_of_ST t s sl0)
+  = ST.tree_req t sl0 <==> tree_req (repr_SF_of_ST t s sl0)
 
 unfold
 let ens_equiv #a #pre #post (t : ST.prog_tree a pre post) (s : ST.prog_shape t)
@@ -429,42 +429,42 @@ let ens_equiv #a #pre #post (t : ST.prog_tree a pre post) (s : ST.prog_shape t)
   : prop
   = ST.tree_ens t sl0 res sl1_ST <==>
    (post_eq_src (post_src_of_shape t s res) sl0 sl1_ST /\
-    tree_ens (repr_Fun_of_ST t s sl0) res (sel_Fun_of_ST post s.shp res sl1_ST))
+    tree_ens (repr_SF_of_ST t s sl0) res (sel_SF_of_ST post s.shp res sl1_ST))
 
 let ens_equiv_rev #a #pre #post (t : ST.prog_tree a pre post) (s : ST.prog_shape t)
-      (sl0 : Fl.flist pre) (res : a) (sl1_Fun : post_v (post_Fun_of_ST post s.shp) res)
-  : Lemma (requires ens_equiv t s sl0 res (sel_ST_of_Fun t s sl0 res sl1_Fun))
-          (ensures  ST.tree_ens t sl0 res (sel_ST_of_Fun t s sl0 res sl1_Fun) <==>
-                    tree_ens (repr_Fun_of_ST t s sl0) res sl1_Fun)
+      (sl0 : Fl.flist pre) (res : a) (sl1_SF : post_v (post_SF_of_ST post s.shp) res)
+  : Lemma (requires ens_equiv t s sl0 res (sel_ST_of_SF t s sl0 res sl1_SF))
+          (ensures  ST.tree_ens t sl0 res (sel_ST_of_SF t s sl0 res sl1_SF) <==>
+                    tree_ens (repr_SF_of_ST t s sl0) res sl1_SF)
   =
     let src = post_src_of_shape t s res in
     let bij = post_bij s.shp            in
-    sell_ST_of_Fun_eq_src src bij sl0 sl1_Fun;
-    sel_Fun_ST_Fun t s sl0 res sl1_Fun
+    sell_ST_of_SF_eq_src src bij sl0 sl1_SF;
+    sel_SF_ST_SF t s sl0 res sl1_SF
 
 
 /// The soundness (and completeness) lemmas:
 
-val repr_Fun_of_ST_req
+val repr_SF_of_ST_req
   (#a : Type u#a) (#pre : ST.pre_t u#b) (#post : ST.post_t u#a u#b a)
   (t : ST.prog_tree a pre post) (s : ST.prog_shape t)
   (sl0 : Fl.flist pre)
   : Lemma (req_equiv t s sl0)
 
-val repr_Fun_of_ST_ens
+val repr_SF_of_ST_ens
   (#a : Type u#a) (#pre : ST.pre_t u#b) (#post : ST.post_t u#a u#b a)
   (t : ST.prog_tree a pre post) (s : ST.prog_shape t)
   (sl0 : Fl.flist pre) (res : a) (sl1 : Fl.flist (post res))
   : Lemma (ens_equiv t s sl0 res sl1)
 
 
-val repr_Fun_of_ST_shape
+val repr_SF_of_ST_shape
   (#a : Type u#a) (#pre : ST.pre_t u#b) (#post : ST.post_t u#a u#b a)
   (t : ST.prog_tree a pre post) (s : ST.prog_shape t)
   (sl0 : Fl.flist pre)
-  : Lemma (prog_has_shape (repr_Fun_of_ST t s sl0) (shape_Fun_of_ST s.shp))
+  : Lemma (prog_has_shape (repr_SF_of_ST t s sl0) (shape_SF_of_ST s.shp))
 
-(*** Steel.Repr.Fun --> Repr.Fun *)
+(*** Steel.Repr.SF --> Repr.Fun *)
 
 (**) val __begin_repr_fun_of_steel : unit
 
@@ -597,7 +597,7 @@ let sl_tys_lam : Fun.tys_lam sl_tys =
 
 (***** Translation of the representation *)
 
-let rec repr_Fun_of_Steel (#val_t : Type u#a) (#sel_t : post_t u#a u#b val_t) (t : prog_tree val_t sel_t)
+let rec repr_Fun_of_SF (#val_t : Type u#a) (#sel_t : post_t u#a u#b val_t) (t : prog_tree val_t sel_t)
   : Tot (Fun.prog_tree u#(max a b + 1) u#(max a (b + 1)) u#(max a (b + 1)) u#a
                        #(sl_tys u#a u#b) ({val_t; sel_t}))
         (decreases t)
@@ -607,28 +607,28 @@ let rec repr_Fun_of_Steel (#val_t : Type u#a) (#sel_t : post_t u#a u#b val_t) (t
   | Tret a x post sl ->
           Fun.Tret #sl_tys ({val_t = a; sel_t = post}) ({vl = x; sl})
   | Tbind a b itm post f g ->
-          Fun.Tbind _ _ (repr_Fun_of_Steel f) (sl_uncurrify (fun x sls -> repr_Fun_of_Steel (g x sls)))
+          Fun.Tbind _ _ (repr_Fun_of_SF f) (sl_uncurrify (fun x sls -> repr_Fun_of_SF (g x sls)))
   | TbindP a b post wp f g ->
-           Fun.TbindP a ({val_t = b; sel_t = post}) wp f (fun (x : a) -> repr_Fun_of_Steel (g x))
+          Fun.TbindP a ({val_t = b; sel_t = post}) wp f (fun (x : a) -> repr_Fun_of_SF (g x))
 
-let rec shape_Fun_of_Steel (#post_n : nat) (s : shape_tree post_n)
+let rec shape_Fun_of_SF (#post_n : nat) (s : shape_tree post_n)
   : Tot (Fun.shape_tree) (decreases s)
   = match s with
   | Sspec _           -> Fun.Sspec
   | Sret  smp_ret _   -> Fun.Sret smp_ret
-  | Sbind _ _ s_f s_g -> Fun.Sbind  (shape_Fun_of_Steel s_f) (shape_Fun_of_Steel s_g)
-  | SbindP  _ s_g     -> Fun.SbindP (shape_Fun_of_Steel s_g)
+  | Sbind _ _ s_f s_g -> Fun.Sbind  (shape_Fun_of_SF s_f) (shape_Fun_of_SF s_g)
+  | SbindP  _ s_g     -> Fun.SbindP (shape_Fun_of_SF s_g)
 
-(***** soundness of Steel.Fun --> Fun *)
+(***** soundness of SF --> Fun *)
 
-val repr_Fun_of_Steel_req (#val_t : Type) (#sel_t : post_t val_t) (t : prog_tree u#a u#b val_t sel_t)
-  : Lemma (tree_req t <==> Fun.tree_req (repr_Fun_of_Steel t))
+val repr_Fun_of_SF_req (#val_t : Type) (#sel_t : post_t val_t) (t : prog_tree u#a u#b val_t sel_t)
+  : Lemma (tree_req t <==> Fun.tree_req (repr_Fun_of_SF t))
 
-val repr_Fun_of_Steel_ens (#val_t : Type) (#sel_t : post_t val_t) (t : prog_tree u#a u#b val_t sel_t)
+val repr_Fun_of_SF_ens (#val_t : Type) (#sel_t : post_t val_t) (t : prog_tree u#a u#b val_t sel_t)
                           (val_v : val_t) (sel_v : Fl.flist (sel_t val_v))
-  : Lemma (tree_ens t val_v sel_v <==> Fun.tree_ens (repr_Fun_of_Steel t) ({val_v; sel_v}))
+  : Lemma (tree_ens t val_v sel_v <==> Fun.tree_ens (repr_Fun_of_SF t) ({val_v; sel_v}))
 
-val repr_Fun_of_Steel_shape
+val repr_Fun_of_SF_shape
       (#val_t : Type) (#sel_t : post_t val_t) (t : prog_tree u#a u#b val_t sel_t)
       (s : prog_shape t)
-  : Lemma (Fun.prog_has_shape (repr_Fun_of_Steel t) (shape_Fun_of_Steel s.shp))
+  : Lemma (Fun.prog_has_shape (repr_Fun_of_SF t) (shape_Fun_of_SF s.shp))
